%tag:0014
%label:":sol:dehnTwistAsSurgery"
%author:JeffHicks
%name:"Dehn twist as surgery"
%type:"solution"

 

 Here, we write $X:=T^*S^n=\{(z_0, \ldots, z_n)\st \sum_{i=0}^n z_i^2=1\}$. Let $f:= \frac{1}{2}\Re\left(\sum_{i=0}^n z_i^2\right)$, and let $g=\frac{1}{2}\Im\left(\sum_{i=0}^n z_i^2\right)$. Then 
 \begin{align*}
    \nabla f = \sum_{i=0}^n x_i \partial_{x_i}- y_i \partial_{y_i} && \nabla g = \sum_{i=0}^n y_i \partial_{x_i} + x_i \partial_{y_i}.
 \end{align*}
The tangent space to $X$ at a point is the orthogonal complement to $\RR \nabla f + \RR \nabla g$. Consider the Hamiltonian 
\begin{align*}
    H: X\to \RR\\
    (\vec x, \vec y )\mapsto \frac{1}{2}|\vec y|^2
\end{align*}
To compute the Hamiltonian flow of $H$, we use that  $V_H=J\circ  \nabla_{X} H$, where $\nabla_X H$ is the gradient of $H$ on $X$ computed with the metric inherited from $\CC^{n+1}$.  We use the following identities:
\begin{align*}
    |\nabla f |^2 = |\vec x|^2+|\vec y|^2 &&  \nabla f \cdot    \nabla g = 0 \\
    \nabla H \cdot \nabla g = 0 && \nabla H \cdot \nabla f = -|\vec y |^2\\
\end{align*}
Computing the gradient by orthogonal projection:
\begin{align*}
    \nabla_X H =& \nabla H - \left(\frac{\nabla f \cdot \nabla H}{|\nabla f|^2}\nabla f \right)\\
    =& \sum_{i=0}^n\left(y_i \partial_{y_i}- \frac{-|\vec y|^2}{|\vec x|^2+ |\vec y|^2}( x_i \partial_{x_i}- y_i \partial_{y_i})\right) \\
    =& \sum_{i=0}^n y_i\left(1- \frac{|\vec y|^2}{|\vec x|^2 +|\vec y|^2}\right) \partial_{y_i}+ \frac{x_i|\vec y|^2}{|\vec x|^2 +|\vec y|^2}\partial_{x_i}\\
    \intertext{Declare $A= |\vec y|^2/(|x|^2+|\vec y|^2)$}
    =& \sum_{i=0}^n \left(1- A\right)y_i\partial_{y_i}+ Ax_i\partial_{x_i}
\end{align*}
Multiplying through by $J$,
\[V_H= \sum_{i=0}^n Ax_i \partial_{y_i} - (1-A)y_i \partial_{x_i}\]
Let $(x_i(t), y_i(t))$ be a Hamiltonian flowline. Then 
\begin{align*}
    x_i'=(1-A) y_i && y_i'=A x_i
\end{align*}
from which we obtain 
\[x_i''=(1-A) A x_i\]
Note that $A$ depends on $y_i$.

For initial conditions $(a_0, \ldots, a_n, b_0, \ldots, b_n)$, set 
\begin{align*}
    A_0 = \frac{|\vec b|^2}{|\vec a|^2 +|\vec b|^2}  && B_0=(1-A_0)A_0
\end{align*}
We guess the solutions
\begin{align*}x_i =& \cos(\sqrt{B_0}t ) a_i + \sin(\sqrt{B_0}t)b_i \\
y_i =& -A_0\sin(\sqrt{B_0}t) a_i  + A_0\cos(\sqrt{B_0}t) b_i
\end{align*}
Observe that $\vec a \cdot \vec b =0$, so 
\[|\vec y(t)|^2=(|\vec a|^2 + |\vec b|^2)\cdot A_0 = |\vec b|^2\]
So, $A(y(t))$ is constant for these guessed solutions. From this we check that the guessed solutions are flowlines of $V_H$.

Observer that at the boundary $|\vec b|=1$, and so  
\begin{align*}
    A_0=1/3 && B_0=2/9
\end{align*}
 Therefore the time $3\pi \sqrt{2}$ flow of $V_H$ acts by mulitplication by $-1$ on the boundary of $X\cap \{(\vec x, \vec y) \st |\vec y|\leq 1\}$.
